ROOT
@@ -1319,6 +1319,7 @@ session RRA_Factor_Structural_Bootstrap = HOL +
     Factor_Required_History_Cases
     Factor_Required_History_Investigation
     Ordered_Finite_Terms
+    Factor_Resolution_Commitments
     Linear_Comparisons
     Prefix_Key_Comparisons
     Ordered_Artifact_Comparison
